theories/sprop.v
@@ -1,68 +1,18 @@
 From Coq Require Export Logic.StrictProp.
-From stdpp Require Import base decidable.
+From stdpp Require Import decidable.
 From stdpp Require Import options.
 
-Definition is_true (b: bool): SProp := if b then sUnit else sEmpty.
+Definition SIs_true (b: bool): SProp := if b then sUnit else sEmpty.
 
-Lemma is_true_intro {b: bool} : Is_true b → is_true b.
-Proof.
-  destruct b; simpl; [ constructor | intros [] ].
-Defined.
+Lemma SIs_true_intro {b: bool} : Is_true b → SIs_true b.
+Proof. destruct b; [constructor | intros []]. Qed.
+Lemma SIs_true_elim {b: bool} : SIs_true b → Is_true b.
+Proof. destruct b; simpl; [constructor | intros []]. Qed.
 
-Lemma is_true_elim {b: bool} : is_true b → Is_true b.
-Proof.
-  destruct b; simpl; [constructor | intros []].
-Defined.
+Definition sprop_decide (P : Prop) `{!Decision P} : SProp :=
+  SIs_true (bool_decide P).
 
-Lemma is_true_fmap {P Q: bool} (lem: P → Q) : is_true P → is_true Q.
-Proof.
-  destruct Q; simpl; [ constructor | ].
-  intros.
-  destruct P; [ | exact H ].
-  exfalso. apply (lem I).
-Defined.
-
-Lemma is_true_bind {P Q: bool} (HP: is_true P) (lem: P → is_true Q) : is_true Q.
-Proof.
-  destruct Q; simpl; [ constructor | ].
-  apply (lem (is_true_elim HP)).
-Defined.
-
-Definition sprop_decide (P: Prop) {dec: Decision P} : SProp :=
-  is_true (bool_decide P).
-
-Lemma sprop_decide_pack (P: Prop) {dec: Decision P} : P → sprop_decide P.
-Proof.
-  intros H.
-  apply is_true_intro; auto using bool_decide_pack.
-Qed.
-Lemma sprop_decide_unpack (P: Prop) {dec: Decision P} : sprop_decide P → P.
-Proof.
-  intros H%is_true_elim.
-  eapply bool_decide_unpack; auto.
-Qed.
-
-(* currently unused; partial progress towards getting coPset to use SProp's Ssig
-rather than sig (with a proof in Prop) *)
-Definition proj1_Ssig {A:Type} {P:A → SProp} (e: Ssig P) : A :=
-  let (a, _) := e in a.
-Definition proj2_Ssig {A:Type} {P:A → SProp} (e: Ssig P) : P (proj1_Ssig e) :=
-  let (_, H) := e in H.
-Lemma Ssig_eq_pi {A:Type} {P:A → SProp}
-      (x y: Ssig P) : x = y ↔ proj1_Ssig x = proj1_Ssig y.
-Proof.
-  split; [intros ->; auto |].
-  destruct x, y; simpl; intros ->; auto.
-Qed.
-(* named after eq_sig_hprop *)
-Lemma eq_Ssig {A:Type} {P:A → SProp}
-      (x y: Ssig P) : proj1_Ssig x = proj1_Ssig y → x = y.
-Proof. apply Ssig_eq_pi. Qed.
-
-Global Instance Ssig_eq_dec {A:Type} {dec: EqDecision A} {P: A → SProp} : EqDecision (Ssig P).
-Proof.
-  intros x y.
-  destruct (decide (proj1_Ssig x = proj1_Ssig y)); [left|right].
-  - apply eq_Ssig; auto.
-  - abstract (intros ->; contradiction).
-Defined.
+Lemma sprop_decide_pack (P : Prop) `{!Decision P} : P → sprop_decide P.
+Proof. intros HP. apply SIs_true_intro, bool_decide_pack, HP. Qed.
+Lemma sprop_decide_unpack (P : Prop) `{!Decision P} : sprop_decide P → P.
+Proof. intros HP. apply (bool_decide_unpack P), SIs_true_elim, HP. Qed.
